commit

AP/AP/FreshA/Fresh1.lean
@@ -24,7 +24,8 @@ theorem AState.even_of_simulate {s s₁ f n} [hs : AState s] [hs₁ : AState s�
 
 theorem AState.fresh1_of_aHwsDisj_aVisited {s fsp} {a : AStrat} [hs : AState s] [ha : a.WF]
 (h : ∀ (d : DStrat) [d.WF], ∀ n, ∃ s₁, sys.simulate (Strat.f ⟨a, d⟩) s (n * 2) = (s₁, 0) ∧
-s₁.aHwsDisj (fsp.offset (n * 2) |>.insertSet 0 # s.aVisited s₁ |>.toSet)) : a.Fresh1 s fsp := by
+s₁.aHwsDisj (fsp.insert 1 s.aPos |>.offset (n * 2) |>.insertSet 0 #
+s.aVisited s₁ |>.toSet.erase s.aPos)) : a.Fresh1 s fsp := by
   use ha
   split_ands
   · intro d hd n
@@ -37,7 +38,11 @@ s₁.aHwsDisj (fsp.offset (n * 2) |>.insertSet 0 # s.aVisited s₁ |>.toSet)) : 
       specialize h₂ default inferInstance 0
       simp at h₂
       simp [FSP.hasLe]
-      exact h₂.2
+      replace h₂ := h₂.2
+      intro k hk
+      specialize h₂ k hk
+      simp [FSP.insert, FSP.insertSet] at h₂
+      grind
     specialize h (n + 1)
     choose s₃ h₃ h₄ using h
     rw [Nat.add_one_mul] at h₃
@@ -53,6 +58,10 @@ s₁.aHwsDisj (fsp.offset (n * 2) |>.insertSet 0 # s.aVisited s₁ |>.toSet)) : 
     specialize h₄ default inferInstance 0
     simp at h₄
     simp [FSP.hasLe]
+    replace h₄ := h₄.2
+    intro k hk
+    specialize h₄ k (by omega)
+    simp [FSP.insert, FSP.insertSet] at h₄
     grind
   intro d hd s₁ p h₁
   specialize h d
@@ -70,7 +79,12 @@ s₁.aHwsDisj (fsp.offset (n * 2) |>.insertSet 0 # s.aVisited s₁ |>.toSet)) : 
   specialize h default inferInstance 0
   simp at h
   simp [h₂] at h₄; subst h₄
-  replace h := h.1
+  have h₆ : s₃.aPos ≠ s.aPos
+  · replace h := h.2
+    specialize h 1 (by omega)
+    simp [FSP.insert, FSP.insertSet] at h
+    exact h.1
+  replace h := h.1 h₆
   have hs₂ := DState.of_tr h₂
   rw [←AState.aPos_eq_of_tr h₂, ←DState.aPos_eq_of_tr h₅]
   simp at h₅
@@ -78,4 +92,142 @@ s₁.aHwsDisj (fsp.offset (n * 2) |>.insertSet 0 # s.aVisited s₁ |>.toSet)) : 
   exact State.aVisited_subset_of_simulate_le ⟨a, d⟩ (n * 2) (n * 2 + 2)
     (by omega) h₁ # by simpa [h₁, h₂]
 
+def aFreshCnd (s : State) (fsp : FSP) (s₁ : State) : Prop :=
+  s₁.aHwsDisj # fsp.offset (s₁.diff s) |>.insertSet 0 # s.aVisited s₁ |>.toSet
+
+noncomputable
+def aFresh (s : State) (fsp : FSP) : AStrat :=
+  aSeek # aFreshCnd s fsp
+
+@[simp]
+instance {s fsp} : aFresh s fsp |>.WF := by
+  unfold aFresh; infer_instance
+
+theorem AState.exi_aSeek_tr {s P} [hs : AState s]
+(h : ∃ p s₁, sys.tr s p = some s₁ ∧ P s₁) :
+∃ s₁, sys.tr s (aSeek P |>.f s) = some s₁ ∧ P s₁ := by
+  simp [aSeek]
+  rw [choose?_eq_of_exi]
+  rotate_left; exact h
+  simp
+  have h₁ := Classical.epsilon_spec h
+  generalize hp : Classical.epsilon (λ p => ∃ s₁, sys.tr s p = some s₁ ∧ P s₁) = p at h₁ ⊢
+  choose s₁ h₁ h₂ using h₁
+  simpa [sys.validTr_of_eq_some h₁, h₁]
+
+theorem AState.aPos_ne_of_tr {s s₁ p} [hs : AState s]
+(h : sys.tr s p = some s₁) : s₁.aPos ≠ s.aPos := by
+  rw [tr_eq_some_iff] at h; grind
+
 -- #check 0 #exit
+
+theorem AState.exi_fresh1_of_aHwsDisj {s fsp} [hs : AState s]
+(h : s.aHwsDisj fsp) : ∃ (a : AStrat), a.Fresh1 s fsp := by
+  use aFresh s fsp
+  apply fresh1_of_aHwsDisj_aVisited
+  intro d hd n
+  replace h := AState.aHwsDisj_insert_one_aPos h
+  induction n
+  ·
+    simp
+    choose a ha h using h
+    use a, ha
+    intro d₁ hd₁ n
+    specialize h d₁ hd₁ n
+    choose s₁ h₁ h₂ using h
+    use s₁, h₁
+    simp [FSP.hasLe, FSP.insert, FSP.insertSet] at h₂ ⊢
+    intro k hk
+    specialize h₂ k hk
+    split_ifs <;> simp_all
+  nm n ih
+  
+  choose s₁ h₁ h₂ using ih
+  simp [Nat.add_one_mul, h₁]
+  
+  have hs₁ := AState.of_simulate_mul_two_eq' h₁
+  
+  generalize h₃ : (fsp.insert 1 s.aPos |>.offset (n * 2) |>.insertSet 0 #
+    s.aVisited s₁ |>.toSet.erase s.aPos) = fsp₁ at h₂
+  
+  replace h₂ := AState.aHwsDisj_insert_one_aPos h₂
+  choose a ha h₂ using h₂
+  
+  obtain ⟨s₂, h₄, h₅⟩ : ∃ s₂, sys.tr s₁ (aFresh s fsp |>.f s₁) = some s₂ ∧ aFreshCnd s fsp s₂
+  ·
+    unfold aFresh
+    apply exi_aSeek_tr
+    
+    choose s₂ h₄ h₅ using h₂ default inferInstance 1
+    
+    simp at h₄
+    use a.f s₁, s₂, h₄
+    
+    -- specialize h₂ d₁ hd₁ (k + 1)
+    -- simp_rw [sys.simulate_succ_full'] at h₂
+    -- simp [h₄] at h₂
+    -- choose s₃ h₂ h₆ using h₂
+    -- use s₃, h₂
+    -- 
+    -- -- cases k
+    -- -- ·
+    -- --   simp at h₆
+    -- --   simp [FSP.hasLe, FSP.insertSet]
+    -- --   split
+    -- 
+    -- -- simp [h₄] at h₂
+    -- -- simp [FSP.hasLe, FSP.insert, FSP.insertSet] at h₂ h₅
+    -- -- specialize h₂ 1
+    -- -- simp [←h₃, FSP.insert, FSP.insertSet] at h₂
+    -- 
+    -- simp [FSP.hasLe]
+    -- intro c hc
+    -- simp [FSP.insertSet]
+    -- 
+    -- have h₇ : s₃.aPos ∉ (fsp.offset # s₂.diff s).get c
+    
+    unfold aFreshCnd
+    rw [State.diff, length_hist_eq_of_tr h₄, State.length_hist_eq_of_simulate_eq h₁]
+    dsimp
+    rw [show s.hist.length + n * 2 + 1 - s.hist.length = n * 2 + 1 by omega]
+    rw [AState.aVisited_eq_of_tr h₄ # sys.reachable_of_simulate_eq h₁]
+    
+    use a, ha
+    intro d₁ hd₁ k
+    specialize h₂ d₁ hd₁ (k + 1)
+    simp only [sys.simulate_succ_full'] at h₂
+    obtain ⟨s₃, ⟨s₂', H₁, H₂⟩, H₃⟩ := h₂
+    simp at H₁
+    
+    simp [h₄] at H₁; subst H₁; clear h₄
+    use s₃, H₂
+    
+    simp [FSP.hasLe, FSP.insert, FSP.insertSet] at H₃ h₅ ⊢
+    intro c hc
+    specialize H₃ (c + 1) (by omega)
+    simp at H₃
+    split_ifs at H₃ ⊢ with H₄
+    ·
+      subst H₄
+      simp at H₃ ⊢
+      rcases H₃ with ⟨H₃, H₄⟩
+      split_ands
+      ·
+        by_contra! H₅
+        sorry
+      ·
+        sorry
+      ·
+        sorry
+    ·
+      sorry
+  
+  simp [h₄]
+  unfold aFreshCnd at h₅
+  
+  -- rw [State.diff, length_hist_eq_of_tr h₄, State.length_hist_eq_of_simulate_eq h₁] at h₅
+  -- dsimp at h₅
+  -- rw [show s.hist.length + n * 2 + 1 - s.hist.length = n * 2 + 1 by omega] at h₅
+  -- rw [AState.aVisited_eq_of_tr h₄ # sys.reachable_of_simulate_eq h₁] at h₅
+  
+  sorry
